Refactored prg assumptions in security analysis

proof/security/MLWE_PKE_Hash.ec
@@ -1,5 +1,5 @@
-require import AllCore Distr List SmtMap Dexcepted PKE_ROM.
-require (****) RndExcept StdOrder MLWE.
+require import AllCore Distr List SmtMap Dexcepted PKE_ROM StdOrder.
+require (**RndExcept **) MLWE PRF.
 
 theory MLWE_PKE_Hash.
 
@@ -43,8 +43,7 @@ op [uniform full lossless]drand : randomness distr.
 
 op prg_kg : randomness -> seed * vector * vector.
 
-axiom prg_kg_correct : 
-   dmap drand prg_kg = 
+op prg_kg_ideal  = 
      dlet dseed
        (fun (sd : seed) => 
           dlet dshort (fun (s : vector) => 
@@ -52,8 +51,7 @@ axiom prg_kg_correct :
 
 op prg_enc : randomness -> vector * vector * R.
 
-axiom prg_enc_correct : 
-   dmap drand prg_enc = 
+op prg_enc_ideal = 
      dlet dshort
        (fun (r : vector) => 
           dlet dshort (fun (e1 : vector) => 
@@ -78,7 +76,7 @@ op dec(sk : skey, c : ciphertext) : plaintext option =
 (******************************************************************)
 (*    The Security Games                                          *)
 
-(* We noe get them from the PKE theory for the UU+TT transformation.
+(* We now get them from the PKE theory for the UU+TT transformation.
 clone import PKE with 
   type pkey <- pkey,
   type skey <- skey,
@@ -195,74 +193,175 @@ module MLWE_PKE_HASH_PROC : Scheme = {
     return (Some (m_decode (v &- (sk_decode sk `<*>` u))));
   }
 }.
+
 (* FIXME : weird parser accepts var (u,v) *)
 
-equiv kg_proc : MLWE_PKE_HASH.kg ~ MLWE_PKE_HASH_PROC.kg : ={arg} ==> ={res}.
-proc.
-transitivity {1} { (pk,sk) <@ MLWE_PKE_HASH_PROC.kg_bridge(); }
-              (true ==> ={pk,sk} )
-              (true ==> pk{1} = pk_encode (sd{2},t{2}) /\ 
-                                sk{1} = sk_encode s{2} ); 1,2:smt().
-+ by inline*; auto; rewrite /kg /= /#.
-inline *. wp 2 3.
-conseq (_: true ==> ={sd,s,e}); 1: by smt(). 
-rndsem*{1} 0.
-rndsem*{2} 0.
-rnd;auto => />;rewrite -prg_kg_correct. 
-have -> : (fun (r0 : randomness) => ((prg_kg r0).`1, (prg_kg r0).`2, (prg_kg r0).`3))
-          = prg_kg; by smt().
-qed.
+(* Equivalence will hold modulo the prgs working correctly *)
 
-equiv enc_proc : MLWE_PKE_HASH.enc ~ MLWE_PKE_HASH_PROC.enc : ={arg} ==> ={res}.
-proc.
-transitivity {1} { c <@ MLWE_PKE_HASH_PROC.enc_bridge(pk,m); }
-              (={pk,m} ==> ={c} )
-              (={pk,m} ==> c{1} = c_encode  (u{2},v{2})); 1,2:smt().
-+ by inline*; auto; smt(). 
-inline *; sp;wp 2 3.
-conseq (_: ={pk,m} ==> ={r,e1,e2}); 1,2: by smt(). 
-rndsem*{1} 0.
-rndsem*{2} 0.
-rnd;auto => />;rewrite -prg_enc_correct. 
-have -> : (fun (rr0 : randomness) => ((prg_enc rr0).`1, (prg_enc rr0).`2, (prg_enc rr0).`3))
-          = prg_enc; by smt().
-qed.
+clone import PRF as PRG_KG with
+   type D <- unit,
+   type R <- seed * vector * vector.
+
+clone import PRG_KG.RF as IDEAL_PRG_KG with
+  op dR <- fun _ => prg_kg_ideal
+  proof dR_ll by admit.
+
+clone import PRG_KG.PseudoRF as REAL_PRG_KG with
+  type K <- randomness,
+  op dK <- drand,
+  op F <- fun k _ => prg_kg k
+  proof dK_ll by admit.
+
+clone import PRF as PRG_ENC with
+   type D <- unit,
+   type R <- vector * vector * R.
+
+clone import PRG_ENC.RF as IDEAL_PRG_ENC with
+  op dR <- fun _ => prg_enc_ideal
+  proof dR_ll by admit.
+
+clone import PRG_ENC.PseudoRF as REAL_PRG_ENC with
+  type K <- randomness,
+  op dK <- drand,
+  op F <- fun k _ => prg_enc k
+  proof dK_ll by admit.
+
+
+module MLWE_PKE_HASH_PRG(KG : PRG_KG.PRF_Oracles, NOISE : PRG_ENC.PRF_Oracles) : Scheme = {
+
+  proc kg() : pkey * skey = {
+     var sd,s,e,t;
+     (sd,s,e) <@ KG.f();
+     t <-  (H sd) *^ s + e;
+     return (pk_encode (sd,t),sk_encode s);
+  }
+
+  proc enc(pk : pkey, m : plaintext) : ciphertext = {
+     var sd,t,r,e1,e2,u,v;
+     (sd,t) <- pk_decode pk;
+     (r,e1,e2) <@ NOISE.f();
+     u <- m_transpose (H sd) *^ r + e1;
+     v <- (t `<*>` r) &+ e2 &+ (m_encode m);
+     return c_encode (u,v);
+  }
+
+  include MLWE_PKE_HASH [dec]
+}.
+
+module (D_KG(A : Adversary) : PRG_KG.Distinguisher) (F : PRG_KG.PRF_Oracles) = {
+   proc distinguish() : bool = {
+       var b;
+       REAL_PRG_ENC.PRF.init();
+       b <@ CPA(MLWE_PKE_HASH_PRG(F,REAL_PRG_ENC.PRF),A).main();
+       return b;
+   }      
+}.
+
+module (D_ENC(A : Adversary) : PRG_ENC.Distinguisher) (F : PRG_ENC.PRF_Oracles) = {
+   proc distinguish() : bool = {
+       var b;
+       IDEAL_PRG_KG.RF.init();
+       b <@ CPA(MLWE_PKE_HASH_PRG(IDEAL_PRG_KG.RF,F),A).main();
+       return b;
+   }      
+}.
 
 section.
 
-declare module A <: Adversary.
+declare module A <: Adversary {-REAL_PRG_KG.PRF, -REAL_PRG_ENC.PRF, -IDEAL_PRG_KG.RF, -IDEAL_PRG_ENC.RF}.
 
 lemma cpa_proc &m : 
-  Pr[CPA(MLWE_PKE_HASH,A).main() @ &m : res] =
-   Pr[CPA(MLWE_PKE_HASH_PROC,A).main() @ &m : res].
+  Pr[CPA(MLWE_PKE_HASH,A).main() @ &m : res] -
+   Pr[CPA(MLWE_PKE_HASH_PROC,A).main() @ &m : res] = 
+     Pr [ PRG_KG.IND(REAL_PRG_KG.PRF,D_KG(A)).main() @ &m : res ] -
+        Pr [ PRG_KG.IND(IDEAL_PRG_KG.RF,D_KG(A)).main() @ &m : res ] +
+     Pr [ PRG_ENC.IND(REAL_PRG_ENC.PRF,D_ENC(A)).main() @ &m : res ] -
+        Pr [ PRG_ENC.IND(IDEAL_PRG_ENC.RF, D_ENC(A)).main() @ &m : res ].
 proof. 
-byequiv => //.
-proc;call(_: true).
-call(enc_proc);rnd.
-call(_: true).
-call(kg_proc).
-by auto.
+have -> : Pr[CPA(MLWE_PKE_HASH,A).main() @ &m : res]  = 
+  Pr [ PRG_KG.IND(REAL_PRG_KG.PRF,D_KG(A)).main() @ &m : res ].
++ byequiv => //.
+  proc;inline *.
+  swap {1} 8 -6. 
+  wp;call(_: true).
+  wp;rnd;call(_: true).
+  by auto => /> /#.
+have -> : Pr[CPA(MLWE_PKE_HASH_PROC, A).main() @ &m : res]   = 
+        Pr[IND(RF, D_ENC(A)).main() @ &m : res].
++ byequiv => //.
+  proc;inline *.
+  rcondt{2} 4; 1: by auto => />;smt(mem_empty).
+  rcondt{2} 15; 1: by auto => />; call(_: true); auto => />;  smt(mem_empty).
+  wp;call(_: true);wp.
+  seq 10 14 : (={glob A,pk,sk,m0,m1,sd0,pk0, t0, m} /\ b{1} = b1{2}) => /=; last first. 
+  + conseq (: _==> r1{2} = (r,e1,e2){1}); 1: by smt(get_setE). 
+    by rndsem{1} 0;auto => /> /#.
+  wp;rnd;call(_:true);wp;sp;conseq(: _==> r0{2} = (sd,s,e){1}); 1: by smt(get_setE).
+  by rndsem{1} 0;auto => /> /#. 
+
+have -> : Pr[PRG_KG.IND(IDEAL_PRG_KG.RF, D_KG(A)).main() @ &m : res] =
+          Pr[IND(PRF, D_ENC(A)).main() @ &m : res]; last by ring.
+by byequiv => //;proc;inline *;swap{1} 1 1;sim.
 qed.
 
 end section.
+
+module (DC_KG(A : CORR_ADV) : PRG_KG.Distinguisher) (F : PRG_KG.PRF_Oracles) = {
+   proc distinguish() : bool = {
+       var b;
+       REAL_PRG_ENC.PRF.init();
+       b <@ Correctness_Adv(MLWE_PKE_HASH_PRG(F,REAL_PRG_ENC.PRF),A).main();
+       return b;
+   }      
+}.
+
+module (DC_ENC(A : CORR_ADV) : PRG_ENC.Distinguisher) (F : PRG_ENC.PRF_Oracles) = {
+   proc distinguish() : bool = {
+       var b;
+       IDEAL_PRG_KG.RF.init();
+       b <@ Correctness_Adv(MLWE_PKE_HASH_PRG(IDEAL_PRG_KG.RF,F),A).main();
+       return b;
+   }      
+}.
+
 
 section.
 
-declare module A <: CORR_ADV.
+declare module A <: CORR_ADV  {-REAL_PRG_KG.PRF, -REAL_PRG_ENC.PRF, -IDEAL_PRG_KG.RF, -IDEAL_PRG_ENC.RF}.
 
 lemma corr_proc &m :
-    Pr[Correctness_Adv(MLWE_PKE_HASH, A).main() @ &m : res] =
-       Pr[Correctness_Adv(MLWE_PKE_HASH_PROC, A).main() @ &m : res].
-byequiv => //.
-proc;call(_: true); 1: by auto;rewrite /dec /#.
-call(enc_proc).
-call(_: true).
-call(kg_proc).
-by auto.
+    Pr[Correctness_Adv(MLWE_PKE_HASH, A).main() @ &m : res] -
+       Pr[Correctness_Adv(MLWE_PKE_HASH_PROC, A).main() @ &m : res] = 
+     Pr [ PRG_KG.IND(REAL_PRG_KG.PRF,DC_KG(A)).main() @ &m : res ] -
+        Pr [ PRG_KG.IND(IDEAL_PRG_KG.RF,DC_KG(A)).main() @ &m : res ] +
+     Pr [ PRG_ENC.IND(REAL_PRG_ENC.PRF,DC_ENC(A)).main() @ &m : res ] -
+        Pr [ PRG_ENC.IND(IDEAL_PRG_ENC.RF, DC_ENC(A)).main() @ &m : res ].
+have -> : Pr[Correctness_Adv(MLWE_PKE_HASH,A).main() @ &m : res]  = 
+  Pr [ PRG_KG.IND(REAL_PRG_KG.PRF,DC_KG(A)).main() @ &m : res ].
++ byequiv => //.
+  proc;inline *.
+  swap {1} 7 -5. 
+  wp;call(_: true).
+  by auto => /> /#.
+have -> : Pr[Correctness_Adv(MLWE_PKE_HASH_PROC, A).main() @ &m : res]   = 
+        Pr[IND(RF, DC_ENC(A)).main() @ &m : res].
++ byequiv => //.
+  proc;inline *.
+  rcondt{2} 4; 1: by auto => />;smt(mem_empty).
+  rcondt{2} 14; 1: by auto => />; call(_: true); auto => />;  smt(mem_empty).
+  wp.
+  seq 9 13 : (={glob A,pk,sk,sd0,pk0, t0, m, m0}) => /=; last first. 
+  + conseq (: _==> r1{2} = (r,e1,e2){1}); 1: by auto => />; smt(get_setE). 
+    by rndsem{1} 0;auto => /> /#.
+  wp;call(_: true);wp;sp;conseq(: _==> r0{2} = (sd,s,e){1}); 1: by smt(get_setE).
+  by rndsem{1} 0;auto => /> /#. 
+
+have -> : Pr[PRG_KG.IND(IDEAL_PRG_KG.RF, DC_KG(A)).main() @ &m : res] =
+          Pr[IND(PRF, DC_ENC(A)).main() @ &m : res]; last by ring.
+by byequiv => //;proc;inline *;swap{1} 1 1;sim.
 qed.
 
 end section.
-
 
 (******************************************************************)
 (*       Game Hopping Security                                    *)
@@ -410,7 +509,7 @@ end section.
 
 section.
 
-declare module A <: Adversary.
+declare module A <: Adversary {-REAL_PRG_KG.PRF, -REAL_PRG_ENC.PRF, -IDEAL_PRG_KG.RF, -IDEAL_PRG_ENC.RF}.
 
 local module Game2(A : Adversary) = {
   proc main() = {
@@ -456,21 +555,25 @@ qed.
 
 lemma main_theorem &m :
   islossless A.guess => islossless A.choose =>
-  Pr[CPA(MLWE_PKE_HASH,A).main() @ &m : res] -  1%r / 2%r =
-    Pr[MLWE_H(B1(A)).main(false,false) @ &m : res] -
-       Pr[MLWE_H(B1(A)).main(false,true) @ &m : res] + 
-    Pr[MLWE_H(B2(A)).main(true,false) @ &m : res] -
-       Pr[MLWE_H(B2(A)).main(true,true) @ &m : res].
+  `| Pr[CPA(MLWE_PKE_HASH,A).main() @ &m : res] -  1%r / 2%r | <=
+    `| Pr[MLWE_H(B1(A)).main(false,false) @ &m : res] -
+       Pr[MLWE_H(B1(A)).main(false,true) @ &m : res] | + 
+    `| Pr[MLWE_H(B2(A)).main(true,false) @ &m : res] -
+       Pr[MLWE_H(B2(A)).main(true,true) @ &m : res] | +
+    `| Pr [ PRG_KG.IND(REAL_PRG_KG.PRF,D_KG(A)).main() @ &m : res ] -
+        Pr [ PRG_KG.IND(IDEAL_PRG_KG.RF,D_KG(A)).main() @ &m : res ] | +
+    `| Pr [ PRG_ENC.IND(REAL_PRG_ENC.PRF,D_ENC(A)).main() @ &m : res ] -
+        Pr [ PRG_ENC.IND(IDEAL_PRG_ENC.RF, D_ENC(A)).main() @ &m : res ] |.
 proof.
 move => A_guess_ll A_choose_ll.
-rewrite (cpa_proc A &m).
+have := (cpa_proc A &m).
 rewrite (hop1_left A &m).
 rewrite (hop1_right A &m).
 rewrite (hop2_left A &m).
 rewrite (hop2_right A &m).
 rewrite (game2_equiv &m).
 rewrite (game2_prob &m _ _) //.
-by ring.
+by smt().
 qed.
 
 end section.
@@ -555,13 +658,20 @@ module CorrectnessAdvNoise(A : CORR_ADV) = {
 
 section.
 
-declare module A <: CORR_ADV.
+declare module A <: CORR_ADV  {-REAL_PRG_KG.PRF, -REAL_PRG_ENC.PRF, -IDEAL_PRG_KG.RF, -IDEAL_PRG_ENC.RF}.
 
 lemma correctness_noise &m:
   Pr[ Correctness_Adv(MLWE_PKE_HASH,A).main() @ &m : res]  <= 
-       Pr[ CorrectnessAdvNoise(A).main() @ &m : res].
+       Pr[ CorrectnessAdvNoise(A).main() @ &m : res] + 
+     Pr [ PRG_KG.IND(REAL_PRG_KG.PRF,DC_KG(A)).main() @ &m : res ] -
+        Pr [ PRG_KG.IND(IDEAL_PRG_KG.RF,DC_KG(A)).main() @ &m : res ] +
+     Pr [ PRG_ENC.IND(REAL_PRG_ENC.PRF,DC_ENC(A)).main() @ &m : res ] -
+        Pr [ PRG_ENC.IND(IDEAL_PRG_ENC.RF, DC_ENC(A)).main() @ &m : res ].
+
 proof.
-rewrite (corr_proc A).
+have  CPROC := (corr_proc A &m).
+have : Pr[Correctness_Adv(MLWE_PKE_HASH_PROC, A).main() @ &m : res] <=
+   Pr[ CorrectnessAdvNoise(A).main() @ &m : res]; last by smt().    
 byequiv => //.
 proc.  
 inline {1} 4. inline {1} 3. inline {1} 1. 
@@ -621,7 +731,8 @@ op noise_exp_part2 _A s e r e2 m =
 
 lemma parts_work _A s e r e1 e2 m :
   noise_exp _A s e r e1 e2 m =
-  noise_exp_part1 _A s e r e1 e2 &+ noise_exp_part2 _A s e r e2 m by rewrite noise_exp_val /noise_exp_simpl /noise_exp_part1 /noise_exp_part2 /=; ring. 
+  noise_exp_part1 _A s e r e1 e2 &+ noise_exp_part2 _A s e r e2 m 
+  by rewrite noise_exp_val /noise_exp_simpl /noise_exp_part1 /noise_exp_part2 /=; ring. 
 
 module CB(A : CORR_ADV) = {
   var s : vector
@@ -682,7 +793,7 @@ module CorrectnessBound = {
 
 section.
 
-declare module A <: CORR_ADV {-CB}.
+declare module A <: CORR_ADV {-CB, -REAL_PRG_KG.PRF, -REAL_PRG_ENC.PRF, -IDEAL_PRG_KG.RF, -IDEAL_PRG_ENC.RF}.
 
 lemma correctness_split &m cv_bound failprob1 failprob2:
   Pr[ CB(A).main() @ &m : 
@@ -731,12 +842,17 @@ qed.
 lemma correctness_theorem &m :
   islossless A.find =>
   Pr[ Correctness_Adv(MLWE_PKE_HASH,A).main() @ &m : res]  <= 
-    Pr[ CorrectnessBound.main() @ &m : res].
+    Pr[ CorrectnessBound.main() @ &m : res] + 
+     `| Pr [ PRG_KG.IND(REAL_PRG_KG.PRF,DC_KG(A)).main() @ &m : res ] -
+        Pr [ PRG_KG.IND(IDEAL_PRG_KG.RF,DC_KG(A)).main() @ &m : res ] | +
+     `| Pr [ PRG_ENC.IND(REAL_PRG_ENC.PRF,DC_ENC(A)).main() @ &m : res ] -
+        Pr [ PRG_ENC.IND(IDEAL_PRG_ENC.RF, DC_ENC(A)).main() @ &m : res ] |.
+
 move => A_ll.
-have := (correctness_split &m cv_bound_max (Pr[ CorrectnessBound.main() @ &m : res]) 0%r _ _).
+have /= CSPLIT := (correctness_split &m cv_bound_max (Pr[ CorrectnessBound.main() @ &m : res]) 0%r _ _).
 + by rewrite (correctness_bound_aux &m A_ll).
 + by have := cv_max &m; smt().
-have := (correctness_noise A &m).
+have CPROC := (correctness_noise A &m).
 by smt().
 qed.
 
@@ -763,7 +879,13 @@ lemma correctness &m fail_prob :
     TT.qHC = 0 =>
     1 < TT.FinT.card =>
     
-Pr[KEMROM.Correctness(KEMROM.RO.RO, FO_K).main() @ &m : res] <= fail_prob.
+Pr[KEMROM.Correctness(KEMROM.RO.RO, FO_K).main() @ &m : res] <= 
+   fail_prob +
+     `| Pr [ PRG_KG.IND(REAL_PRG_KG.PRF,DC_KG(TT.B(B_UC, RO.RO))).main() @ &m : res ] -
+        Pr [ PRG_KG.IND(IDEAL_PRG_KG.RF,DC_KG(TT.B(B_UC, RO.RO))).main() @ &m : res ] | +
+     `| Pr [ PRG_ENC.IND(REAL_PRG_ENC.PRF,DC_ENC(TT.B(B_UC, RO.RO))).main() @ &m : res ] -
+        Pr [ PRG_ENC.IND(IDEAL_PRG_ENC.RF, DC_ENC(TT.B(B_UC, RO.RO))).main() @ &m : res ] |.
+
 proof.
 move => cb qHC0 msp2.
 have := (correctness_fo_k &m qHC0 msp2).
@@ -783,7 +905,7 @@ qed.
 section. 
 
 declare module A <:
-    KEMROM.CCA_ADV{ -KEMROM.RO.RO.m, -OW_CPA, -BOWp, -OWL_CPA, -OWvsIND.Bowl, -RO.RO, -RO.FRO, -OW_PCVA, -TT.BasePKE, -TT.B, -TT.Correctness_Adv1, -TT.CountO, -TT.O_AdvOW, -TT.Gm, -RF.RF, -PseudoRF.PRF, -KEMROMx2.RO1.RO, -KEMROMx2.RO1.FRO, -KEMROMx2.RO2.RO, -KEMROMx2.RO2.FRO, -KEMROMx2.CCA, -CountHx2, -RO1E.FunRO, -UU2, -H2, -H2BOWMod, -Gm2, -Gm3, -KEMROM.CCA, -B1x2, -CB}.
+    KEMROM.CCA_ADV{ -KEMROM.RO.RO.m, -OW_CPA, -BOWp, -OWL_CPA, -OWvsIND.Bowl, -RO.RO, -RO.FRO, -OW_PCVA, -TT.BasePKE, -TT.B, -TT.Correctness_Adv1, -TT.CountO, -TT.O_AdvOW, -TT.Gm, -RF.RF, -PseudoRF.PRF, -KEMROMx2.RO1.RO, -KEMROMx2.RO1.FRO, -KEMROMx2.RO2.RO, -KEMROMx2.RO2.FRO, -KEMROMx2.CCA, -CountHx2, -RO1E.FunRO, -UU2, -H2, -H2BOWMod, -Gm2, -Gm3, -KEMROM.CCA, -B1x2, -CB, -REAL_PRG_KG.PRF, -REAL_PRG_ENC.PRF, -IDEAL_PRG_KG.RF, -IDEAL_PRG_ENC.RF}.
 
 
 module BUOOOWMod_Hx2 = CountH(B1x2(A, CountHx2(BUUOWMod(B1x2(A), TT.CountH(TT.H(TT.CO1(RO.RO))), TT.CountO(TT.G2_O(TT.CO1(RO.RO)))).H2B), KEMROMx2.CCA(CountHx2(BUUOWMod(B1x2(A), TT.CountH(TT.H(TT.CO1(RO.RO))), TT.CountO(TT.G2_O(TT.CO1(RO.RO)))).H2B), UU2, B1x2(A)).O).BH).
@@ -799,9 +921,39 @@ module BUUC_Hx2 = CountH(B1x2(A, CountHx2(BUUC(B1x2(A), TT.CO1(RO.RO)).H2B), KEM
 module BUUC_dec =  KEMROMx2.CCA(CountHx2(BUUC(B1x2(A), TT.CO1(RO.RO)).H2B), UU2, B1x2(A)).O.
 
 
-lemma conclusion &m fail_prob :
+lemma conclusion &m fail_prob prg_kg_bound prg_enc_bound :
     
     Pr[ CorrectnessBound.main() @ &m : res] <= fail_prob =>
+
+   `| Pr[PRG_KG.IND(REAL_PRG_KG.PRF, DC_KG(BOWp(TT.BasePKE, TT.AdvOW_query(BUUOWMod(B1x2(A)))))).main() @ &m : res] -
+       Pr[PRG_KG.IND(IDEAL_PRG_KG.RF, DC_KG(BOWp(TT.BasePKE, TT.AdvOW_query(BUUOWMod(B1x2(A)))))).main() @ &m : res] | <= prg_kg_bound =>
+   `| Pr[PRG_KG.IND(REAL_PRG_KG.PRF, DC_KG(BOWp(TT.BasePKE, TT.AdvOW(BUUOWMod(B1x2(A)))))).main() @ &m : res] -
+       Pr[PRG_KG.IND(IDEAL_PRG_KG.RF, DC_KG(BOWp(TT.BasePKE, TT.AdvOW(BUUOWMod(B1x2(A)))))).main() @ &m : res]  | <= prg_kg_bound =>
+   `| Pr[PRG_KG.IND(REAL_PRG_KG.PRF, DC_KG(TT.B(TT.AdvCorr(BUUOWMod(B1x2(A))), RO.RO))).main() @ &m : res] -
+       Pr[PRG_KG.IND(IDEAL_PRG_KG.RF, DC_KG(TT.B(TT.AdvCorr(BUUOWMod(B1x2(A))), RO.RO))).main() @ &m : res]  | <= prg_kg_bound =>
+   `| Pr[PRG_KG.IND(REAL_PRG_KG.PRF, DC_KG(TT.B(BUUCI(B1x2(A)), RO.RO))).main() @ &m : res] -
+       Pr[PRG_KG.IND(IDEAL_PRG_KG.RF, DC_KG(TT.B(BUUCI(B1x2(A)), RO.RO))).main() @ &m : res]  | <= prg_kg_bound =>
+   `| Pr[PRG_KG.IND(REAL_PRG_KG.PRF, DC_KG(TT.B(BUUC(B1x2(A)), RO.RO))).main() @ &m : res] -
+       Pr[PRG_KG.IND(IDEAL_PRG_KG.RF, DC_KG(TT.B(BUUC(B1x2(A)), RO.RO))).main() @ &m : res]  | <= prg_kg_bound =>
+   `|Pr[PRG_KG.IND(REAL_PRG_KG.PRF, D_KG(OWvsIND.Bowl(OWvsIND.BL(TT.AdvOW(BUUOWMod(B1x2(A))))))).main() @ &m : res] -
+       Pr[PRG_KG.IND(IDEAL_PRG_KG.RF, D_KG(OWvsIND.Bowl(OWvsIND.BL(TT.AdvOW(BUUOWMod(B1x2(A))))))).main() @ &m : res]| <=  prg_kg_bound =>
+   `|Pr[PRG_KG.IND(REAL_PRG_KG.PRF, D_KG(OWvsIND.Bowl(TT.AdvOWL_query(BUUOWMod(B1x2(A)))))).main() @ &m : res] -
+       Pr[PRG_KG.IND(IDEAL_PRG_KG.RF, D_KG(OWvsIND.Bowl(TT.AdvOWL_query(BUUOWMod(B1x2(A)))))).main() @ &m : res]|  <=  prg_kg_bound =>
+   `| Pr[PRG_ENC.IND(PRF, DC_ENC(BOWp(TT.BasePKE, TT.AdvOW_query(BUUOWMod(B1x2(A)))))).main() @ &m : res] -
+       Pr[PRG_ENC.IND(RF, DC_ENC(BOWp(TT.BasePKE, TT.AdvOW_query(BUUOWMod(B1x2(A)))))).main() @ &m : res]|  <= prg_enc_bound =>
+   `| Pr[PRG_ENC.IND(PRF, DC_ENC(BOWp(TT.BasePKE, TT.AdvOW(BUUOWMod(B1x2(A)))))).main() @ &m : res] -
+       Pr[PRG_ENC.IND(RF, DC_ENC(BOWp(TT.BasePKE, TT.AdvOW(BUUOWMod(B1x2(A)))))).main() @ &m : res] |  <= prg_enc_bound =>
+   `| Pr[PRG_ENC.IND(PRF, DC_ENC(TT.B(TT.AdvCorr(BUUOWMod(B1x2(A))), RO.RO))).main() @ &m : res] -
+       Pr[PRG_ENC.IND(RF, DC_ENC(TT.B(TT.AdvCorr(BUUOWMod(B1x2(A))), RO.RO))).main() @ &m : res] |  <= prg_enc_bound =>
+   `| Pr[PRG_ENC.IND(PRF, DC_ENC(TT.B(BUUCI(B1x2(A)), RO.RO))).main() @ &m : res] -
+       Pr[PRG_ENC.IND(RF, DC_ENC(TT.B(BUUCI(B1x2(A)), RO.RO))).main() @ &m : res] |  <= prg_enc_bound =>
+   `| Pr[PRG_ENC.IND(PRF, DC_ENC(TT.B(BUUC(B1x2(A)), RO.RO))).main() @ &m : res] -
+       Pr[PRG_ENC.IND(RF, DC_ENC(TT.B(BUUC(B1x2(A)), RO.RO))).main() @ &m : res] |  <= prg_enc_bound =>
+   `|Pr[IND(PRF, D_ENC(OWvsIND.Bowl(OWvsIND.BL(TT.AdvOW(BUUOWMod(B1x2(A))))))).main() @ &m : res] -
+       Pr[IND(RF, D_ENC(OWvsIND.Bowl(OWvsIND.BL(TT.AdvOW(BUUOWMod(B1x2(A))))))).main() @ &m : res]|  <= prg_enc_bound =>
+   `|Pr[IND(PRF, D_ENC(OWvsIND.Bowl(TT.AdvOWL_query(BUUOWMod(B1x2(A)))))).main() @ &m : res] -
+       Pr[IND(RF, D_ENC(OWvsIND.Bowl(TT.AdvOWL_query(BUUOWMod(B1x2(A)))))).main() @ &m : res]|   <= prg_enc_bound =>
+
 
     qHT = qHK =>
     qHU = qHK =>
@@ -818,19 +970,21 @@ lemma conclusion &m fail_prob :
        islossless O.dec => islossless H0.get => islossless A(H0, O).guess) =>
 
     `|Pr[KEMROM.CCA(KEMROM.RO.RO, FO_K, A).main() @ &m : res] - 1%r / 2%r| <=
-    2%r * `| Pr[MLWE_H(B1(OWvsIND.Bowl(TT.AdvOWL_query(BUUOWMod(B1x2(A)))))).main(false, false) @ &m : res] -
-             Pr[MLWE_H(B1(OWvsIND.Bowl(TT.AdvOWL_query(BUUOWMod(B1x2(A)))))).main(false, true) @ &m : res] +
-             Pr[MLWE_H(B2(OWvsIND.Bowl(TT.AdvOWL_query(BUUOWMod(B1x2(A)))))).main(true, false) @ &m : res] -
-             Pr[MLWE_H(B2(OWvsIND.Bowl(TT.AdvOWL_query(BUUOWMod(B1x2(A)))))).main(true, true) @ &m : res] | +
-    2%r * `| Pr[MLWE_H(B1(OWvsIND.Bowl(OWvsIND.BL(TT.AdvOW(BUUOWMod(B1x2(A))))))).main(false, false) @ &m : res] -
-             Pr[MLWE_H(B1(OWvsIND.Bowl(OWvsIND.BL(TT.AdvOW(BUUOWMod(B1x2(A))))))).main(false, true) @ &m : res] +
-             Pr[MLWE_H(B2(OWvsIND.Bowl(OWvsIND.BL(TT.AdvOW(BUUOWMod(B1x2(A))))))).main(true, false) @ &m : res] -
+    2%r * (`| Pr[MLWE_H(B1(OWvsIND.Bowl(TT.AdvOWL_query(BUUOWMod(B1x2(A)))))).main(false, false) @ &m : res] -
+             Pr[MLWE_H(B1(OWvsIND.Bowl(TT.AdvOWL_query(BUUOWMod(B1x2(A)))))).main(false, true) @ &m : res] | +
+          `| Pr[MLWE_H(B2(OWvsIND.Bowl(TT.AdvOWL_query(BUUOWMod(B1x2(A)))))).main(true, false) @ &m : res] -
+             Pr[MLWE_H(B2(OWvsIND.Bowl(TT.AdvOWL_query(BUUOWMod(B1x2(A)))))).main(true, true) @ &m : res] | + 
+             prg_kg_bound + prg_enc_bound) +
+    2%r * (`| Pr[MLWE_H(B1(OWvsIND.Bowl(OWvsIND.BL(TT.AdvOW(BUUOWMod(B1x2(A))))))).main(false, false) @ &m : res] -
+             Pr[MLWE_H(B1(OWvsIND.Bowl(OWvsIND.BL(TT.AdvOW(BUUOWMod(B1x2(A))))))).main(false, true) @ &m : res] | +
+           `| Pr[MLWE_H(B2(OWvsIND.Bowl(OWvsIND.BL(TT.AdvOW(BUUOWMod(B1x2(A))))))).main(true, false) @ &m : res] -
              Pr[MLWE_H(B2(OWvsIND.Bowl(OWvsIND.BL(TT.AdvOW(BUUOWMod(B1x2(A))))))).main(true, true) @ &m : res]| +
-    (3%r * (2*qHK + 3)%r + 2%r) * fail_prob +
+            prg_kg_bound + prg_enc_bound) +
+    (3%r * (2*qHK + 3)%r + 2%r) * (fail_prob + prg_kg_bound + prg_enc_bound) +
     `|Pr[J.IND(PseudoRF.PRF, D(B1x2(A))).main() @ &m : res] - Pr[J.IND(RF.RF, D(B1x2(A))).main() @ &m : res]| +
     2%r * (2*qHK + 2)%r * eps_msg.
 proof.
-move => fail_probE qhthk qhuhk qvals qv0 qp0 qhv qhcsmall A_count A_ll.
+move => fail_probE kb1 kb2 kb3 kb4 kb5 kb6 kb7 eb1 eb2 eb3 eb4 eb5 eb6 eb7 qhthk qhuhk qvals qv0 qp0 qhv qhcsmall A_count A_ll.
 
 have := conclusion_fo_kyber A &m qhthk qhuhk qvals qv0 qp0 qhv qhcsmall A_count A_ll.
 
@@ -855,7 +1009,10 @@ have <- :
    1: by conseq />;call kg_same;auto => />.
   by inline *;sim.
 
-move => ?.
+move => Htemp.
+have : Pr[TT.PKE.Correctness_Adv(TT.BasePKE, BOWp(TT.BasePKE, TT.AdvOW_query(BUUOWMod(B1x2(A))))).main() @ &m : res] <=
+   Pr[CorrectnessBound.main() @ &m : res] + prg_kg_bound + prg_enc_bound by smt().
+clear Htemp kb1 eb1 => kb1.
 
 have := correctness_theorem (BOWp(TT.BasePKE, TT.AdvOW(BUUOWMod(B1x2(A))))) &m _; 1: by islossless.
 have <- : 
@@ -865,7 +1022,10 @@ have <- :
    1: by conseq />;call kg_same;auto => />.
   by inline *;sim.
 
-move => ?. 
+move => Htemp.
+have : Pr[TT.PKE.Correctness_Adv(TT.BasePKE, BOWp(TT.BasePKE, TT.AdvOW(BUUOWMod(B1x2(A))))).main() @ &m : res] <=
+   Pr[CorrectnessBound.main() @ &m : res] + prg_kg_bound + prg_enc_bound by smt().
+clear Htemp kb2 eb2 => kb2.
 
 have := correctness_theorem (TT.B(TT.AdvCorr(BUUOWMod(B1x2(A))), RO.RO)) &m _.
 +  islossless; last by smt(drange_ll TT.ge0_qH).
@@ -878,7 +1038,10 @@ have <- :
    1: by conseq />;call kg_same;auto => />.
   by inline *;sim.
 
-move => ?. 
+move => Htemp. 
+have : Pr[TT.PKE.Correctness_Adv(TT.BasePKE, TT.B(TT.AdvCorr(BUUOWMod(B1x2(A))), RO.RO)).main() @ &m : res] <=
+   Pr[CorrectnessBound.main() @ &m : res] + prg_kg_bound + prg_enc_bound by smt().
+clear Htemp kb3 eb3 => kb3.
 
 have := correctness_theorem (TT.B(BUUCI(B1x2(A)), RO.RO)) &m _.
 +  islossless; last by smt(drange_ll TT.ge0_qH).
@@ -890,7 +1053,10 @@ have <- :
    1: by conseq />;call kg_same;auto => />.
   by inline *;sim.
 
-move => ?. 
+move => Htemp. 
+have : Pr[TT.PKE.Correctness_Adv(TT.BasePKE, TT.B(BUUCI(B1x2(A)), RO.RO)).main() @ &m : res]  <=
+   Pr[CorrectnessBound.main() @ &m : res] + prg_kg_bound + prg_enc_bound by smt().
+clear Htemp kb4 eb4 => kb4.
 
 have := correctness_theorem (TT.B(BUUC(B1x2(A)), RO.RO)) &m _.
 +  islossless; last by smt(drange_ll TT.ge0_qH).
@@ -903,17 +1069,37 @@ have <- :
    1: by conseq />;call kg_same;auto => />.
   by inline *;sim.
 
-move => ?.
+move => Htemp. 
+have : Pr[TT.PKE.Correctness_Adv(TT.BasePKE, TT.B(BUUC(B1x2(A)), RO.RO)).main() @ &m : res]   <=
+   Pr[CorrectnessBound.main() @ &m : res] + prg_kg_bound + prg_enc_bound by smt().
+clear Htemp kb5 eb5 => kb5.
 
 have := main_theorem (OWvsIND.Bowl(OWvsIND.BL(TT.AdvOW(BUUOWMod(B1x2(A)))))) &m _ _.
 + islossless.
    by apply(A_ll BUOOOWModCPA_Hx2 BUOOOWModCPA_dec);islossless.
 + by islossless.
+
+move => Htemp. 
+have : `|Pr[TT.PKE.CPA(MLWE_PKE_HASH, OWvsIND.Bowl(OWvsIND.BL(TT.AdvOW(BUUOWMod(B1x2(A)))))).main() @ &m : res] -
+         1%r / 2%r| <=
+       `|Pr[MLWE_H(B1(OWvsIND.Bowl(OWvsIND.BL(TT.AdvOW(BUUOWMod(B1x2(A))))))).main(false, false) @ &m : res] -
+         Pr[MLWE_H(B1(OWvsIND.Bowl(OWvsIND.BL(TT.AdvOW(BUUOWMod(B1x2(A))))))).main(false, true) @ &m : res]| +
+       `|Pr[MLWE_H(B2(OWvsIND.Bowl(OWvsIND.BL(TT.AdvOW(BUUOWMod(B1x2(A))))))).main(true, false) @ &m : res] -
+         Pr[MLWE_H(B2(OWvsIND.Bowl(OWvsIND.BL(TT.AdvOW(BUUOWMod(B1x2(A))))))).main(true, true) @ &m : res]| +  prg_kg_bound + prg_enc_bound by smt().
+clear Htemp kb6 eb6 => kb6.
+
 have := main_theorem (OWvsIND.Bowl(TT.AdvOWL_query(BUUOWMod(B1x2(A))))) &m _ _.
-search drange.
 + islossless; last by smt(drange_ll ge0_qHT ge0_qHU) .
    by apply(A_ll BUOOOWModCPA_Hx2 BUOOOWModCPA_dec);islossless.
 + by islossless.
+
+move => Htemp. 
+have : `|Pr[TT.PKE.CPA(MLWE_PKE_HASH, OWvsIND.Bowl(TT.AdvOWL_query(BUUOWMod(B1x2(A))))).main() @ &m : res] - 1%r / 2%r| <=
+       `|Pr[MLWE_H(B1(OWvsIND.Bowl(TT.AdvOWL_query(BUUOWMod(B1x2(A)))))).main(false, false) @ &m : res] -
+         Pr[MLWE_H(B1(OWvsIND.Bowl(TT.AdvOWL_query(BUUOWMod(B1x2(A)))))).main(false, true) @ &m : res]| +
+       `|Pr[MLWE_H(B2(OWvsIND.Bowl(TT.AdvOWL_query(BUUOWMod(B1x2(A)))))).main(true, false) @ &m : res] -
+         Pr[MLWE_H(B2(OWvsIND.Bowl(TT.AdvOWL_query(BUUOWMod(B1x2(A)))))).main(true, true) @ &m : res]| +   prg_kg_bound + prg_enc_bound by smt().
+clear Htemp kb7 eb7 => kb7.
 
 by smt(ge0_qHU ge0_qHT). 
 qed.
